lib/Cast.v
@@ -1,0 +1,74 @@
+Require Import Program.
+Require Import CoqlibC.
+Require Import Any.
+
+Set Implicit Arguments.
+
+
+
+Class LeibEq (A B: Type) := { leibeq: A = B }.
+Arguments LeibEq: clear implicits.
+Definition cast_sigT (a: Any) (B: Type) `{LeibEq (projT1 a) B}: B.
+  rewrite <- leibeq. destruct a. simpl. auto.
+Defined.
+(* Global Program Instance LeibEq_rev (A B: Type) `{LeibEq A B}: LeibEq B A. *)
+(* Next Obligation. rewrite leibeq. eauto. Defined. *)
+Program Definition LeibEq_rev (A B: Type) (LEQ: LeibEq A B): LeibEq B A.
+Proof. rewrite leibeq. econstructor. refl. Defined.
+Definition cast (A B: Type) `{LeibEq A B} (a: A): B. rewrite <- leibeq. apply a. Defined.
+Global Program Instance LeibEq_refl (A: Type): LeibEq A A.
+
+Lemma cast_sigT_existT
+      (x: Any) X
+      (TY: LeibEq (projT1 x) X)
+  :
+    x = existT id _ (@cast_sigT x X TY)
+.
+Proof.
+  destruct x. destruct TY. ss. clarify.
+Qed.
+
+Lemma cast_sigT_eq
+      Y (x: Any) (y: Y)
+      (JMEQ: projT2 x ~= y)
+      (LEIBEQ: LeibEq (projT1 x) Y)
+  :
+    cast_sigT x = y
+.
+Proof.
+  unfold cast_sigT. unfold eq_rect_r. ss. des_ifs. ss.
+  unfold eq_rect. des_ifs.
+Qed.
+
+Lemma cast_sigT_proj
+      Y (x: Any) (y: Y)
+      (LEIBEQ: LeibEq (projT1 x) Y)
+      (EQ: cast_sigT x = y)
+  :
+      <<JMEQ: projT2 x ~= y>>
+.
+Proof.
+  unfold cast_sigT in *. ss. des_ifs. ss. unfold eq_rect. des_ifs.
+Qed.
+
+Lemma cast_elim
+      A LEQ (a: A)
+  :
+    <<EQ: (@cast A A LEQ a) = a>>
+.
+Proof.
+  r. destruct LEQ.
+  unfold cast. ss.
+  unfold eq_rect. dependent destruction leibeq0. ss.
+Qed.
+
+Lemma unit_JMeq
+      X (x: X)
+      (TY: X = unit)
+  :
+    <<EQ: x ~= tt>>
+.
+Proof.
+  revert x. rewrite TY.
+  ii. clarify.
+Qed.
